finish proof for radix tree

src/dict.v
@@ -1,1 +1,93 @@
+Require Import Bool.
+Require Import ZArith.
+Require Import Zdiv.
+Require Import Coq.Lists.List.
+Import ListNotations.
+Require Import radix.
+Require Import utils.
+
+Section Dict.
+  Variable A: Set.
+  Variable eq: A -> A -> bool.
+  Variable eq_spec: forall x y : A, reflect (x = y) (eq x y).
+  Variable B: Set.
+
+  Variable hash: A -> positive.
+
+  Definition t := tree (list (A * B)).
+
+  Definition empty : t := empty.
+
+  Definition find (k: A) (d: t): option B :=
+    match get (hash k) d with
+    | None   => None
+    | Some l => find_snd A B (fun '(k', _) => eq k k') l
+    end.
+
+  Definition add (k: A) (e: B) (d: t): t := 
+    let h_k := hash k in
+    match get h_k d with
+    | None   => set h_k [(k, e)] d
+    | Some l => set h_k ((k, e)::l) d
+    end.
+
+  Theorem dempty:
+    forall (k: A), find k empty = None.
+  Proof.
+    intro i. unfold find. 
+    assert (get (hash i) empty = None).
+    apply gempty. now rewrite H.
+  Qed.
+
+  Theorem dss: 
+    forall (k: A) (x: B) (d: t), find k (add k x d) = Some x.
+  Proof.
+    intros k x d. unfold find, add.
+    case (get (hash k) d).
+    - intro l. rewrite gss. simpl. 
+      case (eq_spec k k). now intro. contradiction.
+    - rewrite gss. simpl.
+      case (eq_spec k k). now intro. contradiction.
+  Qed.
+
+  Lemma hash_equal:
+    forall (k1 k2: A) (x: B) (d: t) (l: list (A * B)),
+      hash k1 = hash k2 -> 
+      get (hash k1) d = Some l -> 
+      get (hash k1) (add k2 x d) = Some ((k2, x) :: l).
+  Proof.
+    intros k1 k2 x d l H Hget.
+    unfold add. rewrite <- H. rewrite Hget.
+    apply gss.
+  Qed.
+
+  Lemma hash_diff:
+    forall (k1 k2: A) (x: B) (d: t) (l: option (list (A *B))),
+      hash k1 <> hash k2 -> 
+      get (hash k1) d = l -> 
+      get (hash k1) (add k2 x d) = l.
+  Proof.
+    intros k1 k2 x d l H Hget. rewrite <- Hget.
+    unfold add. case (get (hash k2) d).
+    intro l0. now apply gso.
+    now apply gso.
+  Qed.
+
+  Theorem dso:
+    forall (k1 k2: A) (x: B) (d: t),
+      k1 <> k2 -> find k1 (add k2 x d) = find k1 d.
+  Proof.
+    intros k1 k2 x d H. unfold find.
+    case (Pos.eq_dec (hash k1) (hash k2)).
+    - intros Heq. 
+      destruct (get (hash k1) d) eqn:Hget.
+      rewrite hash_equal with (1 := Heq) (2 := Hget). 
+      simpl. case (eq_spec k1 k2). easy. now intros _.
+      rewrite Heq. unfold add.
+      rewrite <- Heq, Hget. rewrite gss. simpl.
+      case (eq_spec k1 k2). easy. now intros _.
+    - intro Hdiff. case (get (hash k1) d) eqn:Hget;
+      now rewrite hash_diff with (1 := Hdiff) (2 := Hget).
+  Qed.
+End Dict.
 
