src/utils.v
@@ -1,0 +1,16 @@
+Require Import Coq.Lists.List.
+Import ListNotations.
+
+Section List.
+  Variable A: Type.
+  Variable B: Type.
+
+  Fixpoint find_snd (f : A * B -> bool) (l :list (A * B)): option B :=
+    match l with
+    | nil     => None
+    | x :: tl => if f x then Some (snd x) else find_snd f tl
+    end.
+End List.
+
+Arguments find_snd : clear implicits.
+
